AwsCryptographicMaterialProviders/runtimes/java/src/examples/java/software/amazon/cryptography/example/hierarchy/CreateKeyExample.java
@@ -1,0 +1,100 @@
+// Copyright Amazon.com Inc. or its affiliates. All Rights Reserved.
+// SPDX-License-Identifier: Apache-2.0
+package software.amazon.cryptography.example.hierarchy;
+
+import java.util.Collections;
+import java.util.Map;
+import javax.annotation.Nonnull;
+import javax.annotation.Nullable;
+import software.amazon.awssdk.services.dynamodb.DynamoDbClient;
+import software.amazon.awssdk.utils.StringUtils;
+import software.amazon.cryptography.keystoreadmin.KeyStoreAdmin;
+import software.amazon.cryptography.keystoreadmin.model.CreateKeyInput;
+import software.amazon.cryptography.keystoreadmin.model.KmsSymmetricKeyArn;
+
+/*
+  The Hierarchical Keyring Example relies on the existence of a
+  key store with pre-existing branch key material or beacon key material.
+
+  This example demonstrates configuring a Key Store Admin and then
+  using a helper method to create a branch key and beacon key
+  that share the same Id, then return that Id.
+  We will always create a new beacon key alongside a new branch key,
+  even if you are not using searchable encryption.
+
+  This key creation should occur within your control plane.
+ */
+public class CreateKeyExample {
+
+  public static String CreateKey(
+    @Nonnull String keyStoreTableName,
+    @Nonnull String logicalKeyStoreName,
+    @Nonnull String kmsKeyArn,
+    @Nullable String branchKeyId,
+    @Nullable DynamoDbClient dynamoDbClient
+  ) {
+    // 1. Configure your Key Store Admin resource.
+    KeyStoreAdmin admin = AdminProvider.admin(
+      keyStoreTableName,
+      logicalKeyStoreName,
+      dynamoDbClient
+    );
+
+    // 2. If you need to specify the Identifier for a Branch Key, you may.
+    // This is an optional argument.
+    // If an Identifier is not provided, a v4 UUID will be generated and used.
+    // This example provides a combination of a fixed string and a v4 UUID;
+    // this makes it easy for Crypto Tools to clean up these Example Branch Keys.
+    branchKeyId =
+      StringUtils.isBlank(branchKeyId)
+        ? "mpl-java-example-" + java.util.UUID.randomUUID().toString()
+        : branchKeyId;
+
+    // 3. Create a custom encryption context for the Branch Key.
+    // Most encrypted data should have an associated encryption context
+    // to protect integrity. This sample uses placeholder values.
+    // Note that the custom encryption context for a Branch Key is
+    // prefixed by the library with `aws-crypto-ec:`.
+    // For more information see:
+    // blogs.aws.amazon.com/security/post/Tx2LZ6WBJJANTNW/How-to-Protect-the-Integrity-of-Your-Encrypted-Data-by-Using-AWS-Key-Management
+    final Map<String, String> encryptionContext = Collections.singletonMap(
+      "ExampleContextKey",
+      "ExampleContextValue"
+    );
+
+    // 2. Create a new branch key and beacon key in our KeyStore.
+    //    Both the branch key and the beacon key will share an Id.
+    //    This creation is eventually consistent.
+    final String actualBranchKeyId = admin
+      .CreateKey(
+        CreateKeyInput
+          .builder()
+          // This is the KMS ARN that will be used to protect the Branch Key.
+          // It is a required argument.
+          .KmsArn(KmsSymmetricKeyArn.builder().KmsKeyArn(kmsKeyArn).build())
+          // If you need to specify the Identifier for a Branch Key, you may.
+          // This is an optional argument.
+          .Identifier(branchKeyId)
+          // If a branch key Identifier is provided,
+          // custom encryption context MUST be provided as well.
+          .EncryptionContext(encryptionContext)
+          .build()
+      )
+      .Identifier();
+
+    assert actualBranchKeyId.equals(branchKeyId);
+    return branchKeyId;
+  }
+
+  public static void main(final String[] args) {
+    if (args.length <= 1) {
+      throw new IllegalArgumentException(
+        "To run this example, include the keyStoreTableName, logicalKeyStoreName, and kmsKeyArn in args"
+      );
+    }
+    final String keyStoreTableName = args[0];
+    final String logicalKeyStoreName = args[1];
+    final String kmsKeyArn = args[2];
+    CreateKey(keyStoreTableName, logicalKeyStoreName, kmsKeyArn, null, null);
+  }
+}
