AwsCryptographicMaterialProviders/runtimes/java/src/main/smithy-generated/software/amazon/cryptography/keystoreadmin/model/CreateKeyInput.java
@@ -1,0 +1,194 @@
+// Copyright Amazon.com Inc. or its affiliates. All Rights Reserved.
+// SPDX-License-Identifier: Apache-2.0
+// Do not modify this file. This file is machine generated, and any changes to it will be overwritten.
+package software.amazon.cryptography.keystoreadmin.model;
+
+import java.util.Map;
+import java.util.Objects;
+
+public class CreateKeyInput {
+
+  /**
+   * The identifier for the created Branch Key.
+   */
+  private final String Identifier;
+
+  /**
+   * Custom encryption context for the Branch Key.
+   *   Required if branchKeyIdentifier is set.
+   */
+  private final Map<String, String> EncryptionContext;
+
+  /**
+   * Multi-Region or Single Region AWS KMS Key
+   *   used to protect the Branch Key, but not aliases!
+   */
+  private final KmsSymmetricKeyArn KmsArn;
+
+  /**
+   * This configures which Key Management Operations will be used
+   *    AND the Key Management Clients (and Grant Tokens) used to invoke those Operations.
+   */
+  private final KeyManagementStrategy Strategy;
+
+  protected CreateKeyInput(BuilderImpl builder) {
+    this.Identifier = builder.Identifier();
+    this.EncryptionContext = builder.EncryptionContext();
+    this.KmsArn = builder.KmsArn();
+    this.Strategy = builder.Strategy();
+  }
+
+  /**
+   * @return The identifier for the created Branch Key.
+   */
+  public String Identifier() {
+    return this.Identifier;
+  }
+
+  /**
+   * @return Custom encryption context for the Branch Key.
+   *   Required if branchKeyIdentifier is set.
+   */
+  public Map<String, String> EncryptionContext() {
+    return this.EncryptionContext;
+  }
+
+  /**
+   * @return Multi-Region or Single Region AWS KMS Key
+   *   used to protect the Branch Key, but not aliases!
+   */
+  public KmsSymmetricKeyArn KmsArn() {
+    return this.KmsArn;
+  }
+
+  /**
+   * @return This configures which Key Management Operations will be used
+   *    AND the Key Management Clients (and Grant Tokens) used to invoke those Operations.
+   */
+  public KeyManagementStrategy Strategy() {
+    return this.Strategy;
+  }
+
+  public Builder toBuilder() {
+    return new BuilderImpl(this);
+  }
+
+  public static Builder builder() {
+    return new BuilderImpl();
+  }
+
+  public interface Builder {
+    /**
+     * @param Identifier The identifier for the created Branch Key.
+     */
+    Builder Identifier(String Identifier);
+
+    /**
+     * @return The identifier for the created Branch Key.
+     */
+    String Identifier();
+
+    /**
+     * @param EncryptionContext Custom encryption context for the Branch Key.
+     *   Required if branchKeyIdentifier is set.
+     */
+    Builder EncryptionContext(Map<String, String> EncryptionContext);
+
+    /**
+     * @return Custom encryption context for the Branch Key.
+     *   Required if branchKeyIdentifier is set.
+     */
+    Map<String, String> EncryptionContext();
+
+    /**
+     * @param KmsArn Multi-Region or Single Region AWS KMS Key
+     *   used to protect the Branch Key, but not aliases!
+     */
+    Builder KmsArn(KmsSymmetricKeyArn KmsArn);
+
+    /**
+     * @return Multi-Region or Single Region AWS KMS Key
+     *   used to protect the Branch Key, but not aliases!
+     */
+    KmsSymmetricKeyArn KmsArn();
+
+    /**
+     * @param Strategy This configures which Key Management Operations will be used
+     *    AND the Key Management Clients (and Grant Tokens) used to invoke those Operations.
+     */
+    Builder Strategy(KeyManagementStrategy Strategy);
+
+    /**
+     * @return This configures which Key Management Operations will be used
+     *    AND the Key Management Clients (and Grant Tokens) used to invoke those Operations.
+     */
+    KeyManagementStrategy Strategy();
+
+    CreateKeyInput build();
+  }
+
+  static class BuilderImpl implements Builder {
+
+    protected String Identifier;
+
+    protected Map<String, String> EncryptionContext;
+
+    protected KmsSymmetricKeyArn KmsArn;
+
+    protected KeyManagementStrategy Strategy;
+
+    protected BuilderImpl() {}
+
+    protected BuilderImpl(CreateKeyInput model) {
+      this.Identifier = model.Identifier();
+      this.EncryptionContext = model.EncryptionContext();
+      this.KmsArn = model.KmsArn();
+      this.Strategy = model.Strategy();
+    }
+
+    public Builder Identifier(String Identifier) {
+      this.Identifier = Identifier;
+      return this;
+    }
+
+    public String Identifier() {
+      return this.Identifier;
+    }
+
+    public Builder EncryptionContext(Map<String, String> EncryptionContext) {
+      this.EncryptionContext = EncryptionContext;
+      return this;
+    }
+
+    public Map<String, String> EncryptionContext() {
+      return this.EncryptionContext;
+    }
+
+    public Builder KmsArn(KmsSymmetricKeyArn KmsArn) {
+      this.KmsArn = KmsArn;
+      return this;
+    }
+
+    public KmsSymmetricKeyArn KmsArn() {
+      return this.KmsArn;
+    }
+
+    public Builder Strategy(KeyManagementStrategy Strategy) {
+      this.Strategy = Strategy;
+      return this;
+    }
+
+    public KeyManagementStrategy Strategy() {
+      return this.Strategy;
+    }
+
+    public CreateKeyInput build() {
+      if (Objects.isNull(this.KmsArn())) {
+        throw new IllegalArgumentException(
+          "Missing value for required field `KmsArn`"
+        );
+      }
+      return new CreateKeyInput(this);
+    }
+  }
+}
