AwsCryptographicMaterialProviders/runtimes/java/src/main/smithy-generated/software/amazon/cryptography/keystoreadmin/model/InitializeMutationInput.java
@@ -1,0 +1,221 @@
+// Copyright Amazon.com Inc. or its affiliates. All Rights Reserved.
+// SPDX-License-Identifier: Apache-2.0
+// Do not modify this file. This file is machine generated, and any changes to it will be overwritten.
+package software.amazon.cryptography.keystoreadmin.model;
+
+import java.util.Objects;
+
+public class InitializeMutationInput {
+
+  /**
+   * The identifier for the Branch Key to be mutated.
+   */
+  private final String Identifier;
+
+  /**
+   * Describes the Mutation that will be applied to all Items of the Branch Key.
+   */
+  private final Mutations Mutations;
+
+  /**
+   * Optional. Defaults to reEncrypt with a default KMS Client.
+   */
+  private final KeyManagementStrategy Strategy;
+
+  /**
+   * Optional. Defaults to TrustStorage. See System Key.
+   */
+  private final SystemKey SystemKey;
+
+  /**
+   * Optional. Defaults to False. As of v1.8.0, setting this true throws a UnsupportedFeatureException.
+   */
+  private final Boolean DoNotVersion;
+
+  protected InitializeMutationInput(BuilderImpl builder) {
+    this.Identifier = builder.Identifier();
+    this.Mutations = builder.Mutations();
+    this.Strategy = builder.Strategy();
+    this.SystemKey = builder.SystemKey();
+    this.DoNotVersion = builder.DoNotVersion();
+  }
+
+  /**
+   * @return The identifier for the Branch Key to be mutated.
+   */
+  public String Identifier() {
+    return this.Identifier;
+  }
+
+  /**
+   * @return Describes the Mutation that will be applied to all Items of the Branch Key.
+   */
+  public Mutations Mutations() {
+    return this.Mutations;
+  }
+
+  /**
+   * @return Optional. Defaults to reEncrypt with a default KMS Client.
+   */
+  public KeyManagementStrategy Strategy() {
+    return this.Strategy;
+  }
+
+  /**
+   * @return Optional. Defaults to TrustStorage. See System Key.
+   */
+  public SystemKey SystemKey() {
+    return this.SystemKey;
+  }
+
+  /**
+   * @return Optional. Defaults to False. As of v1.8.0, setting this true throws a UnsupportedFeatureException.
+   */
+  public Boolean DoNotVersion() {
+    return this.DoNotVersion;
+  }
+
+  public Builder toBuilder() {
+    return new BuilderImpl(this);
+  }
+
+  public static Builder builder() {
+    return new BuilderImpl();
+  }
+
+  public interface Builder {
+    /**
+     * @param Identifier The identifier for the Branch Key to be mutated.
+     */
+    Builder Identifier(String Identifier);
+
+    /**
+     * @return The identifier for the Branch Key to be mutated.
+     */
+    String Identifier();
+
+    /**
+     * @param Mutations Describes the Mutation that will be applied to all Items of the Branch Key.
+     */
+    Builder Mutations(Mutations Mutations);
+
+    /**
+     * @return Describes the Mutation that will be applied to all Items of the Branch Key.
+     */
+    Mutations Mutations();
+
+    /**
+     * @param Strategy Optional. Defaults to reEncrypt with a default KMS Client.
+     */
+    Builder Strategy(KeyManagementStrategy Strategy);
+
+    /**
+     * @return Optional. Defaults to reEncrypt with a default KMS Client.
+     */
+    KeyManagementStrategy Strategy();
+
+    /**
+     * @param SystemKey Optional. Defaults to TrustStorage. See System Key.
+     */
+    Builder SystemKey(SystemKey SystemKey);
+
+    /**
+     * @return Optional. Defaults to TrustStorage. See System Key.
+     */
+    SystemKey SystemKey();
+
+    /**
+     * @param DoNotVersion Optional. Defaults to False. As of v1.8.0, setting this true throws a UnsupportedFeatureException.
+     */
+    Builder DoNotVersion(Boolean DoNotVersion);
+
+    /**
+     * @return Optional. Defaults to False. As of v1.8.0, setting this true throws a UnsupportedFeatureException.
+     */
+    Boolean DoNotVersion();
+
+    InitializeMutationInput build();
+  }
+
+  static class BuilderImpl implements Builder {
+
+    protected String Identifier;
+
+    protected Mutations Mutations;
+
+    protected KeyManagementStrategy Strategy;
+
+    protected SystemKey SystemKey;
+
+    protected Boolean DoNotVersion;
+
+    protected BuilderImpl() {}
+
+    protected BuilderImpl(InitializeMutationInput model) {
+      this.Identifier = model.Identifier();
+      this.Mutations = model.Mutations();
+      this.Strategy = model.Strategy();
+      this.SystemKey = model.SystemKey();
+      this.DoNotVersion = model.DoNotVersion();
+    }
+
+    public Builder Identifier(String Identifier) {
+      this.Identifier = Identifier;
+      return this;
+    }
+
+    public String Identifier() {
+      return this.Identifier;
+    }
+
+    public Builder Mutations(Mutations Mutations) {
+      this.Mutations = Mutations;
+      return this;
+    }
+
+    public Mutations Mutations() {
+      return this.Mutations;
+    }
+
+    public Builder Strategy(KeyManagementStrategy Strategy) {
+      this.Strategy = Strategy;
+      return this;
+    }
+
+    public KeyManagementStrategy Strategy() {
+      return this.Strategy;
+    }
+
+    public Builder SystemKey(SystemKey SystemKey) {
+      this.SystemKey = SystemKey;
+      return this;
+    }
+
+    public SystemKey SystemKey() {
+      return this.SystemKey;
+    }
+
+    public Builder DoNotVersion(Boolean DoNotVersion) {
+      this.DoNotVersion = DoNotVersion;
+      return this;
+    }
+
+    public Boolean DoNotVersion() {
+      return this.DoNotVersion;
+    }
+
+    public InitializeMutationInput build() {
+      if (Objects.isNull(this.Identifier())) {
+        throw new IllegalArgumentException(
+          "Missing value for required field `Identifier`"
+        );
+      }
+      if (Objects.isNull(this.Mutations())) {
+        throw new IllegalArgumentException(
+          "Missing value for required field `Mutations`"
+        );
+      }
+      return new InitializeMutationInput(this);
+    }
+  }
+}
