AwsCryptographicMaterialProviders/runtimes/java/src/main/smithy-generated/software/amazon/cryptography/keystoreadmin/model/KmsSymmetricEncryption.java
@@ -1,0 +1,99 @@
+// Copyright Amazon.com Inc. or its affiliates. All Rights Reserved.
+// SPDX-License-Identifier: Apache-2.0
+// Do not modify this file. This file is machine generated, and any changes to it will be overwritten.
+package software.amazon.cryptography.keystoreadmin.model;
+
+import java.util.Objects;
+import software.amazon.cryptography.keystore.model.AwsKms;
+
+/**
+ * Items of non-cryptographic material nature are protected by KMS.
+ * This is done by including all attributes of an item as Encryption Context
+ * in a KMS Encrypt or Decrypt call,
+ * effectively signing the attributes.
+ */
+public class KmsSymmetricEncryption {
+
+  private final KmsSymmetricKeyArn KmsArn;
+
+  private final AwsKms AwsKms;
+
+  protected KmsSymmetricEncryption(BuilderImpl builder) {
+    this.KmsArn = builder.KmsArn();
+    this.AwsKms = builder.AwsKms();
+  }
+
+  public KmsSymmetricKeyArn KmsArn() {
+    return this.KmsArn;
+  }
+
+  public AwsKms AwsKms() {
+    return this.AwsKms;
+  }
+
+  public Builder toBuilder() {
+    return new BuilderImpl(this);
+  }
+
+  public static Builder builder() {
+    return new BuilderImpl();
+  }
+
+  public interface Builder {
+    Builder KmsArn(KmsSymmetricKeyArn KmsArn);
+
+    KmsSymmetricKeyArn KmsArn();
+
+    Builder AwsKms(AwsKms AwsKms);
+
+    AwsKms AwsKms();
+
+    KmsSymmetricEncryption build();
+  }
+
+  static class BuilderImpl implements Builder {
+
+    protected KmsSymmetricKeyArn KmsArn;
+
+    protected AwsKms AwsKms;
+
+    protected BuilderImpl() {}
+
+    protected BuilderImpl(KmsSymmetricEncryption model) {
+      this.KmsArn = model.KmsArn();
+      this.AwsKms = model.AwsKms();
+    }
+
+    public Builder KmsArn(KmsSymmetricKeyArn KmsArn) {
+      this.KmsArn = KmsArn;
+      return this;
+    }
+
+    public KmsSymmetricKeyArn KmsArn() {
+      return this.KmsArn;
+    }
+
+    public Builder AwsKms(AwsKms AwsKms) {
+      this.AwsKms = AwsKms;
+      return this;
+    }
+
+    public AwsKms AwsKms() {
+      return this.AwsKms;
+    }
+
+    public KmsSymmetricEncryption build() {
+      if (Objects.isNull(this.KmsArn())) {
+        throw new IllegalArgumentException(
+          "Missing value for required field `KmsArn`"
+        );
+      }
+      if (Objects.isNull(this.AwsKms())) {
+        throw new IllegalArgumentException(
+          "Missing value for required field `AwsKms`"
+        );
+      }
+      return new KmsSymmetricEncryption(this);
+    }
+  }
+}
