AwsCryptographicMaterialProviders/dafny/AwsCryptographyKeyStore/test/Storage/TestQueryForVersions.dfy
@@ -1,0 +1,93 @@
+// Copyright Amazon.com Inc. or its affiliates. All Rights Reserved.
+// SPDX-License-Identifier: Apache-2.0
+
+include "../Fixtures.dfy"
+include "../CleanupItems.dfy"
+
+module {:options "/functionSyntax:4"} TestQueryForVersions {
+  import Fixtures
+  import UInt = Fixtures.UInt
+  import Types = Fixtures.Types
+  import UTF8 = Fixtures.UTF8
+  import DDB = Com.Amazonaws.Dynamodb
+  import KMS = Com.Amazonaws.Kms
+  import Time
+  import CleanupItems
+  import opened Wrappers
+  import String = StandardLibrary.String
+  import Structure
+
+  const ddbTableName: DDB.Types.TableName := Fixtures.branchKeyStoreName
+  const logicalKeyStoreName := Fixtures.logicalKeyStoreName
+  const happyCaseId := "test-query-for-versions"
+
+  method {:test} TestHappyCase()
+  {
+    print " running";
+    var ddbClient :- expect DDB.DynamoDBClient();
+    var underTest :- expect Fixtures.DefaultStorage(ddbClient?:=Some(ddbClient));
+    // TODO-Mutations-GA restore tests once done refactoring storage
+    // var inputQuery: Types.QueryForVersionsInput;
+    // var items: Types.EncryptedHierarchicalKeys;
+    // var startKey: seq<UInt.uint8>;
+    // var queryOut : Types.QueryForVersionsOutput;
+    // var strStartKey: string;
+
+    // inputQuery := Types.QueryForVersionsInput(
+    //   Identifier := happyCaseId,
+    //   PageSize := 2
+    // );
+
+    // var pageLimit := 3;
+    // var pageIndex := 0;
+    // var queryCount := 0;
+    // while pageIndex < pageLimit
+    // {
+
+    //   print "\nTestQueryForVersions :: TestHappyCase :: pre-Query "
+    //         + String.Base10Int2String(queryCount+1)  +
+    //         " :: Input Start Key is None? :: " +
+    //         (if inputQuery.ExclusiveStartKey.None? then "True" else "False")
+    //         + "\n";
+    //   assume {:axiom} underTest.Modifies == {}; // Turns off verification
+    //   queryOut :- expect underTest.QueryForVersions(inputQuery);
+    //   queryCount := queryCount + 1;
+    //   items := queryOut.Items;
+    //   startKey := queryOut.ExclusiveStartKey;
+    //   strStartKey := "";
+
+    //   if (|items| > 0) {
+    //     expect
+    //       |items| == 2,
+    //       "Query returned items but not 2 of them? Size of items: " + String.Base10Int2String(|items|);
+    //     var strItems: seq<string> := seq(|items|, (i: nat) requires i < |items| => items[i].EncryptionContext[Structure.TYPE_FIELD]);
+    //     print "\nTestQueryForVersions :: TestHappyCase :: Query "
+    //           + String.Base10Int2String(queryCount)  +  " :: Items :: "
+    //           + strItems[0] + " , " + strItems[1] + "\n";
+    //   }
+
+    //   if (|startKey| > 0) {
+    //     strStartKey :- expect UTF8.Decode(startKey);
+    //     print "\nTestQueryForVersions :: TestHappyCase :: Query "
+    //           + String.Base10Int2String(queryCount)  +  " :: Start Key :: " + strStartKey + "\n";
+    //   } else {
+    //     strStartKey := "";
+    //     print "\nTestQueryForVersions :: TestHappyCase :: Query "
+    //           + String.Base10Int2String(queryCount)  +  " :: Did not have a start key.\n";
+    //     pageIndex := 10; // Short cut
+    //   }
+
+    //   inputQuery := Types.QueryForVersionsInput(
+    //     Identifier := inputQuery.Identifier,
+    //     PageSize := inputQuery.PageSize,
+    //     ExclusiveStartKey := if |startKey| > 0 then Some(startKey) else None()
+    //   );
+    //   pageIndex := pageIndex + 1;
+    // }
+
+    // expect
+    //   queryCount == 2,
+    //   "It should have take 2 queries to fetch all versions, but it did not!";
+    print "TestQueryForVersions.TestHappyCase: ";
+  }
+}
