AwsCryptographicMaterialProviders/dafny/AwsCryptographyKeyStoreAdmin/src/PrefixUtils.dfy
@@ -1,0 +1,48 @@
+// Copyright Amazon.com Inc. or its affiliates. All Rights Reserved.
+// SPDX-License-Identifier: Apache-2.0
+
+module {:options "/functionSyntax:4" } PrefixUtils {
+  // import opened Structure
+
+  opaque function AddingPrefixToKeysOfMapDoesNotCreateCollisions(
+    nameonly prefix: string,
+    nameonly aMap: map<string, string>
+  ): (output: map<string, string>)
+    ensures forall k <- aMap
+              ::
+                && prefix + k in output
+                && output[prefix + k] == aMap[k]
+  {
+    // Dafny needs some help.
+    // Adding a fixed string
+    // will not make any of the keys collide.
+    // However, this leaks a lot of complexity.
+    // This is why the function is now opaque.
+    // Otherwise things timeout
+    assert forall k <- aMap.Keys
+        ::
+          k == (prefix + k)[|prefix|..];
+
+    map k <- aMap :: prefix + k := aMap[k]
+  }
+
+  opaque function FilterMapForKeysThatDoNotBeginWithPrefix (
+    nameonly prefix: string,
+    nameonly aMap: map<string, string>
+  ): (output: map<string, string>)
+    ensures forall k <- output
+              ::
+                && !( prefix < k)
+                && k in aMap
+                && output[k] == aMap[k]
+  {
+    var filteredKeys
+      :=
+      set k <- aMap
+          | !(prefix < k)
+        ::
+          k;
+    map i <- filteredKeys :: i := aMap[i]
+  }
+
+}
